DRT for partial eval/auth and roundtrip proof
Signed-off-by: Aaron Eline <aeline+github@amazon.com>

cedar-drt/fuzz/fuzz_targets/partial-auth.rs
@@ -1,0 +1,128 @@
+/*
+ * Copyright Cedar Contributors
+ *
+ * Licensed under the Apache License, Version 2.0 (the "License");
+ * you may not use this file except in compliance with the License.
+ * You may obtain a copy of the License at
+ *
+ *      https://www.apache.org/licenses/LICENSE-2.0
+ *
+ * Unless required by applicable law or agreed to in writing, software
+ * distributed under the License is distributed on an "AS IS" BASIS,
+ * WITHOUT WARRANTIES OR CONDITIONS OF ANY KIND, either express or implied.
+ * See the License for the specific language governing permissions and
+ * limitations under the License.
+ */
+
+#![no_main]
+use cedar_drt::*;
+use cedar_drt_inner::fuzz_target;
+use cedar_drt_inner::*;
+use cedar_policy_core::ast::Context;
+use cedar_policy_core::ast::Effect;
+use cedar_policy_core::ast::Expr;
+use cedar_policy_core::ast::Policy;
+use cedar_policy_core::ast::PolicyID;
+use cedar_policy_core::ast::PolicySet;
+use cedar_policy_core::ast::Request;
+use cedar_policy_core::ast::RestrictedExpr;
+use cedar_policy_core::entities::Entities;
+use cedar_policy_core::extensions::Extensions;
+use cedar_testing::cedar_test_impl::RustEngine;
+use libfuzzer_sys::arbitrary::{self, Arbitrary, Unstructured};
+use serde::Serialize;
+
+#[derive(Debug, Clone, Serialize)]
+struct FuzzTargetInput {
+    policies: PolicySet,
+}
+
+#[derive(Debug, Clone)]
+pub struct PolicySpec {
+    effect: Effect,
+    kind: PolicyKind,
+}
+
+impl PolicySpec {
+    pub fn policy(&self, id: String) -> Policy {
+        let when = match self.kind {
+            PolicyKind::True => Expr::val(true),
+            PolicyKind::False => Expr::val(false),
+            PolicyKind::Error => Expr::add(Expr::val(1), Expr::val(false)),
+            PolicyKind::Residual => Expr::get_attr(Expr::var(ast::Var::Context), "unknown".into()),
+        };
+        Policy::from_when_clause(self.effect, when, PolicyID::from_string(id), None)
+    }
+}
+
+impl Arbitrary<'_> for PolicySpec {
+    fn arbitrary(u: &mut Unstructured<'_>) -> arbitrary::Result<Self> {
+        let effect = u.arbitrary()?;
+        let kind = u.arbitrary()?;
+        Ok(Self { effect, kind })
+    }
+}
+
+#[derive(Debug, Clone, Copy, Arbitrary)]
+enum PolicyKind {
+    True,
+    False,
+    Error,
+    Residual,
+}
+
+impl Arbitrary<'_> for FuzzTargetInput {
+    fn arbitrary(u: &mut Unstructured<'_>) -> arbitrary::Result<Self> {
+        let mut policies = PolicySet::new();
+
+        let len = u.arbitrary_len::<PolicySpec>()?;
+
+        for i in 0..len {
+            let id = format!("{i}");
+            let spec: PolicySpec = u.arbitrary()?;
+            let policy = spec.policy(id);
+            policies.add(policy).unwrap();
+        }
+
+        Ok(Self { policies })
+    }
+}
+
+fn build_request() -> Request {
+    let principal = r#"Principal::"alice""#.parse().unwrap();
+    let action = r#"Action::"read""#.parse().unwrap();
+    let resource = r#"Resource::"photo""#.parse().unwrap();
+    use std::iter::once;
+    let context = Context::from_pairs(
+        once((
+            "unknown".into(),
+            RestrictedExpr::call_extension_fn(
+                "unknown".parse().unwrap(),
+                once(RestrictedExpr::val("a")),
+            ),
+        )),
+        Extensions::all_available(),
+    )
+    .unwrap();
+
+    Request::new::<cedar_policy_core::ast::RequestSchemaAllPass>(
+        (principal, None),
+        (action, None),
+        (resource, None),
+        context,
+        None,
+        Extensions::all_available(),
+    )
+    .unwrap()
+}
+
+fuzz_target! {|input: FuzzTargetInput| {
+        let request = build_request();
+        let entities = Entities::new();
+        let def_impl = LeanDefinitionalEngine::new();
+        let prod_impl = RustEngine::new();
+        let def_answer = def_impl.partial_is_authorized(&request, &entities, &input.policies).expect("Lean engine failed to produce a repsonse: ");
+        let prod_answer = prod_impl.partial_is_authorized(&request, &entities, &input.policies).expect("Rust engine failed to produce a response: ");
+        assert_eq!(def_answer, prod_answer);
+    }
+}
