cedar-lean/Cedar/Thm/Partial/Expr/Lemmas.lean
@@ -1,0 +1,587 @@
+/-
+ Copyright Cedar Contributors
+
+ Licensed under the Apache License, Version 2.0 (the "License");
+ you may not use this file except in compliance with the License.
+ You may obtain a copy of the License at
+
+      https://www.apache.org/licenses/LICENSE-2.0
+
+ Unless required by applicable law or agreed to in writing, software
+ distributed under the License is distributed on an "AS IS" BASIS,
+ WITHOUT WARRANTIES OR CONDITIONS OF ANY KIND, either express or implied.
+ See the License for the specific language governing permissions and
+ limitations under the License.
+-/
+
+import Cedar.Partial.Expr
+import Cedar.Thm.Data.List
+import Cedar.Spec
+import Cedar.Thm.Data.Applicative
+
+namespace Cedar.Partial.Thm.Expr
+
+
+/--
+  `List.mapM_pmap_subtype` specialized for a particular setting involving attribute pairs
+-/
+private theorem mapM_pmap_subtype_partial_attr
+  {p : (Spec.Attr × β) → Prop}
+  (f : β → Option Spec.Expr)
+  (pairs: List (Spec.Attr × β))
+  (h : ∀ pair ∈ pairs, p pair) :
+  List.mapM (λ x : {pair : (Spec.Attr × β) // p pair} =>
+    Option.map (λ e => (x.val.fst, e)) (f x.val.snd)) (List.pmap Subtype.mk pairs h) =
+  pairs.mapM (λ x => Option.map (λ e => (x.fst, e)) (f x.snd))
+:= by
+  rw [←List.mapM'_eq_mapM]
+  induction pairs <;> simp [*]
+
+/--
+  `List.map_pmap_subtype` specialized for a particular setting involving attribute pairs
+-/
+private theorem map_pmap_subtype_attr
+  {p : (Spec.Attr × β) → Prop}
+  (f : β → Partial.Expr)
+  (pairs : List (Spec.Attr × β))
+  (h : ∀ pair ∈ pairs, p pair) :
+  List.map (λ x : {pair : (Spec.Attr × β) // p pair} => (x.val.fst, f x.val.snd)) (List.pmap Subtype.mk pairs h) =
+  pairs.map (λ x => (x.fst, f x.snd))
+  := by
+  induction pairs <;> simp [*]
+
+
+/--
+  `List.mapM₂_eq_mapM` specialized for a particular setting involving attribute pairs
+-/
+private theorem mapM₂_eq_mapM_partial_attr [SizeOf β]
+  (f : β → Option Spec.Expr)
+  (attrs : List (Spec.Attr × β)) :
+  attrs.mapM₂
+    (λ x : {x : Spec.Attr × β // sizeOf x.snd < 1 + sizeOf attrs} => match x with
+      | ⟨(a, b), _⟩ => Option.map (λ e => (a, e)) (f b)
+    ) =
+  attrs.mapM λ (a, b) => Option.map (λ e => (a, e)) (f b)
+:= by
+  simp [List.mapM₂, List.attach₂, mapM_pmap_subtype_partial_attr]
+
+/--
+  `List.mapM₂_eq_mapM` specialized for a particular setting involving attribute pairs
+-/
+private theorem map_attach_eq_map_attr [SizeOf β]
+  (f : β → Partial.Expr)
+  (attrs : List (Spec.Attr × β)) :
+  List.map
+    (λ x : {x : Spec.Attr × β // sizeOf x.snd < 1 + sizeOf attrs} => match x with
+      | ⟨(a,b), _ ⟩ => (a, f b)
+    ) (List.attach₂ attrs) =
+  List.map (λ (a,b) => (a, f b)) attrs
+  := by
+  simp [List.map, List.attach₂, map_pmap_subtype_attr]
+
+/--
+  Tactic for proving roundtrip property for binary operation nodes
+-/
+local macro "binary_node" roundtrip:ident : tactic => do
+  `(tactic | (
+    rename_i lhs rhs h
+    unfold Partial.Expr.asSpec at ( h )
+    cases h_lhs : Partial.Expr.asSpec lhs
+    case _ =>
+      rw [h_lhs] at ( h )
+      simp only [Option.map_eq_map, Option.map_none'] at ( h )
+      rw [applicative_none] at ( h )
+      contradiction
+      rfl
+    case _ lhs' =>
+      cases h_rhs : Partial.Expr.asSpec rhs
+      case _ =>
+        rw [h_rhs] at ( h )
+        simp only [Option.map_eq_map] at ( h )
+        rw [applicative_of_none] at ( h )
+        contradiction
+        rfl
+      case _ rhs' =>
+        have ih_lhs : lhs'.asPartialExpr = ( lhs ) := $roundtrip lhs lhs'  h_lhs
+        have ih_rhs : rhs'.asPartialExpr = ( rhs ) := $roundtrip rhs rhs' h_rhs
+        rw [h_lhs] at ( h )
+        rw [h_rhs] at ( h )
+        simp only [Option.map_eq_map, Option.map_some'] at ( h )
+        rw [applicative_step] at ( h )
+        injection ( h )
+        rename_i h
+        rw [← h]
+        unfold Spec.Expr.asPartialExpr
+        rw [ih_lhs]
+        rw [ih_rhs]
+  ))
+
+/--
+  Tactic for proving roundtrip property for unary op
+-/
+local macro "unary_simple" h:ident arg:ident roundtrip:ident : tactic => do
+  `(tactic |  (
+    unfold Partial.Expr.asSpec at ( $h )
+    cases h_arg : Partial.Expr.asSpec $arg
+    case _ =>
+      rw [h_arg] at ( $h )
+      simp at ( $h )
+
+    case _ arg' =>
+      rw [h_arg] at ( $h )
+      simp at ( $h )
+      have ih : arg'.asPartialExpr = $arg := $roundtrip $arg arg' h_arg
+      rw [← $h]
+      unfold Spec.Expr.asPartialExpr
+      rw [ih]
+  ))
+
+/--
+  Tactic for proving roundtrip property for get/has attr
+-/
+local macro "attr" roundtrip:ident : tactic => do
+    `(tactic | (
+    rename_i arg a h
+    unfold Partial.Expr.asSpec at ( h )
+    cases h_arg : Partial.Expr.asSpec arg
+    case _ =>
+      rw [h_arg] at ( h )
+      simp at ( h )
+      rw [applicative_none] at ( h )
+      simp at ( h )
+      rw [applicative_none] at ( h )
+      contradiction
+    case _ arg' =>
+      rw [h_arg] at ( h )
+      simp at ( h )
+      have ih : arg'.asPartialExpr = arg := $roundtrip arg arg' h_arg
+      rw [applicative_step] at ( h )
+      injection ( h )
+      rename_i h
+      rw [← h]
+      unfold Spec.Expr.asPartialExpr
+      rw [ih]))
+
+
+theorem roundtrip₁ : ∀ (pe : Partial.Expr) (e : Spec.Expr),
+  (pe.asSpec = some e) →
+  e.asPartialExpr = pe
+  := by
+  intros pe e h
+  cases pe
+    <;> (try (attr roundtrip₁))
+    <;> (try (binary_node roundtrip₁))
+    <;> try (unfold Partial.Expr.asSpec at h
+            <;> injection h
+            <;> rename_i h
+            <;> rw [← h]
+            <;> unfold Spec.Expr.asPartialExpr
+            <;> rfl)
+  case ite cond cons alt =>
+    unfold Partial.Expr.asSpec at h
+    cases h_cond : cond.asSpec <;> rw [h_cond] at h
+    case none =>
+      simp only [Option.map_eq_map, Option.map_none'] at h
+      rw [applicative_none] at h
+      ·
+        contradiction
+      ·
+        apply applicative_none
+        rfl
+    case some cond' =>
+      cases h_cons : cons.asSpec  <;> rw [h_cons ] at h
+      case none =>
+        simp only [Option.map_eq_map, Option.map_some'] at h
+        have inner : ((some (Spec.Expr.ite cond')) <*> none) = none := by
+          apply applicative_of_none
+          rfl
+        rw [inner] at h
+        rw [applicative_none] at h
+        contradiction
+        rfl
+      case some cons' =>
+        cases h_alt : alt.asSpec <;> rw [h_alt] at h
+        case none =>
+          simp at h
+          rw [applicative_of_none] at h
+          contradiction
+          rfl
+        case some alt' =>
+          have ih_cond : cond'.asPartialExpr = cond := roundtrip₁ cond cond' h_cond
+          have ih_cons : cons'.asPartialExpr = cons := roundtrip₁ cons cons' h_cons
+          have ih_alt : alt'.asPartialExpr = alt := roundtrip₁ alt alt' h_alt
+          simp only [Option.map_eq_map, Option.map_some'] at h
+          have inner₁ : (some (Spec.Expr.ite cond')) <*> (some cons') = some (Spec.Expr.ite cond' cons') := by
+            apply applicative_some
+            repeat rfl
+          rw [inner₁] at h
+          have inner₂ : (some (Spec.Expr.ite cond' cons')) <*> (some alt') = some (Spec.Expr.ite cond' cons' alt') := by
+            apply applicative_some
+            repeat rfl
+          rw [inner₂] at h
+          injection h
+          rename_i h
+          rw [← h]
+          unfold Spec.Expr.asPartialExpr
+          rw [ih_cond]
+          rw [ih_cons]
+          rw [ih_alt]
+  case unaryApp o arg =>
+    unary_simple h arg roundtrip₁
+  case set members =>
+    have inner : ∀ (es : List Partial.Expr) (es' : List Spec.Expr),
+      sizeOf es < sizeOf (Partial.Expr.set members) →
+      List.mapM Partial.Expr.asSpec es = some es' →
+      List.map Spec.Expr.asPartialExpr es' = es
+      := by
+        intros es
+        induction es
+        case nil =>
+          intros es' _  h₂
+          simp only [List.mapM_nil, Option.pure_def, Option.some.injEq] at h₂
+          rw [← h₂]
+          simp
+        case cons head tail ih =>
+          intros es' h₁ h₂
+          simp only [List.mapM_cons, Option.pure_def, Option.bind_eq_bind, Option.bind_eq_some,
+            Option.some.injEq] at h₂
+          have ⟨ head', h_head, tail', h_tail, h_eq ⟩ := h₂
+          rw [← h_eq]
+          simp only [List.map_cons, List.cons.injEq]
+          apply And.intro
+          case _ =>
+            exact roundtrip₁ head head' h_head
+          case _ =>
+            apply ih <;> try assumption
+            simp only [Partial.Expr.set.sizeOf_spec]
+            simp only [List.cons.sizeOf_spec, Partial.Expr.set.sizeOf_spec] at h₁
+            omega
+    unfold Partial.Expr.asSpec at h
+    rw [List.mapM₁_eq_mapM] at h
+    simp only [Option.map_eq_map, Option.map_eq_some'] at h
+    have ⟨ members', h₁ , h₂ ⟩ := h
+    rw [← h₂]
+    unfold Spec.Expr.asPartialExpr
+    rw [List.map₁_eq_map]
+
+    have sizeH : sizeOf members < sizeOf (Partial.Expr.set members) := by
+      simp only [Partial.Expr.set.sizeOf_spec]
+      omega
+    rw [inner]
+    repeat assumption
+  case record attrs =>
+    have inner : ∀ (es : List (Spec.Attr × Partial.Expr)) (es' : List (Spec.Attr × Spec.Expr)),
+      sizeOf es < sizeOf (Partial.Expr.record attrs) →
+      List.mapM (λ pair => Option.map (λ e => (pair.fst, e)) pair.snd.asSpec) es = some es' →
+      List.map (λ pair => (pair.fst, pair.snd.asPartialExpr)) es' = es := by
+      intros es
+      induction es
+      case _ =>
+        intros es _ h₂
+        simp only [List.mapM_nil, Option.pure_def, Option.some.injEq] at h₂
+        rw [← h₂]
+        simp only [List.map_nil]
+      case cons head tail ih =>
+        intros es h₁ h₂
+        simp only [List.mapM_cons, Option.pure_def, Option.bind_eq_bind, Option.bind_eq_some,
+          Option.map_eq_some', Option.some.injEq] at h₂
+        have ⟨ head', h_head, tail', h_tail, h_eq ⟩ := h₂
+        rw [← h_eq]
+        simp only [List.map_cons, List.cons.injEq]
+        apply And.intro
+        ·
+          have ⟨ e', h_head₁, h_head₂ ⟩ := h_head
+          rw [← h_head₂]
+          simp only
+          have eq : Spec.Expr.asPartialExpr e' = head.snd := roundtrip₁ head.snd e' h_head₁
+          rw [eq]
+        ·
+          apply ih
+          simp only [List.cons.sizeOf_spec, Partial.Expr.record.sizeOf_spec] at h₁
+          simp only [Partial.Expr.record.sizeOf_spec]
+          omega
+          assumption
+    unfold Partial.Expr.asSpec at h
+    simp only [Option.map_eq_map, Option.map_eq_some'] at h
+    have ⟨ attrs', h₁, h₂ ⟩ := h
+    rw [← h₂]
+    unfold Spec.Expr.asPartialExpr
+
+    rw [mapM₂_eq_mapM_partial_attr] at h₁
+    rw [map_attach_eq_map_attr]
+    have size_h : sizeOf attrs < sizeOf (Partial.Expr.record attrs) := by
+      simp only [Partial.Expr.record.sizeOf_spec]
+      omega
+    rw [inner]
+    repeat assumption
+  case call xfn args =>
+    have inner : ∀ (es : List Partial.Expr) (es' : List Spec.Expr),
+      sizeOf es < sizeOf (Partial.Expr.call xfn args) →
+      List.mapM Partial.Expr.asSpec es = some es' →
+      List.map Spec.Expr.asPartialExpr es' = es
+      := by
+        intros es
+        induction es
+        case nil =>
+          intros es' _ h₂
+          simp only [List.mapM_nil, Option.pure_def, Option.some.injEq] at h₂
+          rw [← h₂]
+          simp
+        case cons head tail ih =>
+          intros es' h₁ h₂
+          simp only [List.mapM_cons, Option.pure_def, Option.bind_eq_bind, Option.bind_eq_some,
+            Option.some.injEq] at h₂
+          have ⟨ head', h_head, tail', h_tail, h_eq ⟩ := h₂
+          rw [← h_eq]
+          simp only [List.map_cons, List.cons.injEq]
+          apply And.intro
+          case _ =>
+            exact roundtrip₁ head head' h_head
+          case _ =>
+            apply ih <;> try assumption
+            simp only [Partial.Expr.call.sizeOf_spec]
+            simp only [List.cons.sizeOf_spec, Partial.Expr.call.sizeOf_spec] at h₁
+            omega
+    unfold Partial.Expr.asSpec at h
+    rw [List.mapM₁_eq_mapM] at h
+    simp only [Option.map_eq_map, Option.map_eq_some'] at h
+    have ⟨ members', h₁ , h₂ ⟩ := h
+    rw [← h₂]
+    unfold Spec.Expr.asPartialExpr
+    rw [List.map₁_eq_map]
+
+    have sizeH : sizeOf args < sizeOf (Partial.Expr.call xfn args) := by
+      simp only [Partial.Expr.call.sizeOf_spec]
+      omega
+    rw [inner]
+    repeat assumption
+termination_by sizeOf pe
+decreasing_by
+  all_goals (try (simp_wf <;> (try rename_i a _ _ _ _ _ _ <;> rw [a]) <;> (try (rename_i a _ _ _ _ _ _ _ <;> rw [a])) <;> (try (rename_i a _ _ _) <;> rw [a]) <;> simp <;> omega))
+  case _ =>
+    simp_wf
+    rename_i f _ _ _
+    rw [f]
+    simp only [Partial.Expr.set.sizeOf_spec]
+    simp at h₁
+    omega
+  case _ =>
+    simp_wf
+    simp only [List.cons.sizeOf_spec, Partial.Expr.record.sizeOf_spec] at h₁
+    rename_i f g _ _
+    rw [f]
+    simp only [Partial.Expr.record.sizeOf_spec]
+    have size_step : sizeOf g.snd < sizeOf g := by
+      cases g
+      case _ =>
+        simp only [Prod.mk.sizeOf_spec]
+        omega
+    omega
+  case _ =>
+    simp_wf
+    rename_i f _ _ _
+    rw [f]
+    simp only [Partial.Expr.call.sizeOf_spec]
+    simp at h₁
+    omega
+
+
+/-
+  Creates an inductive hypothesis for the given expression
+-/
+local macro "roundtrip₂_recurse" r:ident e:ident : tactic => do
+  `(tactic| (
+    have ih : Expr.asSpec (Spec.Expr.asPartialExpr $e) = some $e := by
+      apply $r
+      rfl
+    rw [ih]
+  ))
+
+/-
+  Domain-specific combination of simps and rfl, repeated
+-/
+local macro "slam" : tactic => do
+  `(tactic |(
+    simp only [Option.map_eq_map, Option.map_some']
+    repeat rw [applicative_some]
+    repeat rfl
+  ))
+
+/-
+  Solves binary ops goals for roundtrip₂
+-/
+local macro "binop₂" r:ident : tactic => do
+  `(tactic | (
+    rename_i lhs rhs
+    roundtrip₂_recurse $r lhs
+    roundtrip₂_recurse $r rhs
+    slam
+  ))
+
+/-
+  Simplify a bunch then call omega
+-/
+local macro "somega" : tactic => do
+  `(tactic | (
+    simp only [
+      List.cons.sizeOf_spec,
+      Spec.Expr.record.sizeOf_spec,
+      Spec.Expr.call.sizeOf_spec,
+      Spec.Expr.set.sizeOf_spec]
+    omega
+  ))
+
+/--
+  A theorem for mapM specialized to option
+-/
+private theorem mapM_option_cons
+  (a : α)
+  (as : List α)
+  (b : β)
+  (bs : List β)
+  (f : α → Option β) :
+  f a = some b →
+  List.mapM f as = some bs  →
+  List.mapM f (a :: as) = some (b :: bs) := by
+  intros h₁ h₂
+  simp
+  apply And.intro <;> assumption
+
+theorem roundtrip₂ : ∀ (e : Spec.Expr) (pe : Partial.Expr),
+  e.asPartialExpr = pe →
+  (pe.asSpec = some e) := by
+  intros e
+  cases e  <;> intros pe h
+    <;> (try (simp only [Spec.Expr.asPartialExpr] at h <;> rw [← h] <;> simp only [Expr.asSpec]))
+    <;> (try (rename_i lhs rhs <;> roundtrip₂_recurse roundtrip₂ lhs <;> roundtrip₂_recurse roundtrip₂ rhs <;> slam))
+    <;> (try (rename_i a _ <;> roundtrip₂_recurse roundtrip₂ a <;> slam))
+    <;> try (repeat rfl)
+  case ite cond cons alt =>
+    roundtrip₂_recurse roundtrip₂ cond
+    slam
+  case unaryApp =>
+    rename_i e
+    roundtrip₂_recurse roundtrip₂ e
+    slam
+  case set members =>
+    have inner : ∀ (es : List Spec.Expr) (es' : List Partial.Expr),
+      sizeOf es < sizeOf (Spec.Expr.set members) →
+      List.map Spec.Expr.asPartialExpr es = es' →
+      List.mapM Partial.Expr.asSpec es' = some es := by
+        intros es
+        induction es <;> intros es' h₁ h₂
+        case nil =>
+          simp only [List.map_nil] at h₂
+          rw [← h₂]
+          simp only [List.mapM_nil, Option.pure_def]
+        case cons head tail ih =>
+          cases es'
+          case nil =>
+            simp only [List.map_cons] at h₂
+          case cons head' tail' =>
+            simp only [List.map_cons, List.cons.injEq] at h₂
+            have ⟨h_head, h_tails ⟩ := h₂
+            rw [mapM_option_cons]
+            apply roundtrip₂
+            assumption
+            apply ih
+            simp only [List.cons.sizeOf_spec, Spec.Expr.set.sizeOf_spec] at h₁
+            somega
+            assumption
+    rw [List.mapM₁_eq_mapM]
+    rw [List.map₁_eq_map]
+    rw [inner]
+    simp only [Option.map_eq_map, Option.map_some', Option.some.injEq, Spec.Expr.set.injEq]
+    rfl
+    somega
+    rfl
+  case record attrs =>
+    simp only [Option.map_eq_map, Option.map_eq_some', Spec.Expr.record.injEq, exists_eq_right]
+    rw [mapM₂_eq_mapM_partial_attr]
+    rw [map_attach_eq_map_attr]
+    have inner : ∀ (as: List (Spec.Attr × Spec.Expr)) (pas: List (Spec.Attr × Partial.Expr)),
+      sizeOf as < sizeOf (Spec.Expr.record attrs) →
+      List.map (λ (name,expr) => (name, expr.asPartialExpr)) as = pas →
+      List.mapM (λ (name,expr) => Option.map (λ e => (name,e)) expr.asSpec) pas = some as
+      := by
+      intros as
+      induction as <;> intros pas h₁ h₂
+      case nil =>
+        simp only [List.map_nil] at h₂
+        rw [← h₂]
+        simp
+      case cons head tail ih =>
+        simp only [List.map_cons] at h₂
+        simp only
+        cases pas
+        case nil =>
+          simp at h₂
+        case cons head' tail' =>
+          simp only [List.cons.injEq] at h₂
+          have ⟨ h₂₁, h₂₂ ⟩ := h₂
+          rw [mapM_option_cons]
+          simp only [Option.map_eq_some']
+          exists head.snd
+          apply And.intro
+          case _ => {
+            apply roundtrip₂
+            rw [← h₂₁]
+          }
+          case _ => {
+            rw [← h₂₁]
+          }
+          case _ => {
+            apply ih
+            simp only [List.cons.sizeOf_spec, Spec.Expr.record.sizeOf_spec] at h₁
+            somega
+            assumption
+          }
+    rw [inner]
+    somega
+    rfl
+  case call xfn args =>
+    have inner : ∀ (es : List Spec.Expr) (es' : List Partial.Expr),
+      sizeOf es < sizeOf (Spec.Expr.call xfn args) →
+      List.map Spec.Expr.asPartialExpr es = es' →
+      List.mapM Partial.Expr.asSpec es' = some es := by
+        intros es
+        induction es <;> intros es' h₁ h₂
+        case nil =>
+          simp only [List.map_nil] at h₂
+          rw [← h₂]
+          simp only [List.mapM_nil, Option.pure_def]
+        case cons head tail ih =>
+          cases es'
+          case nil =>
+            simp only [List.map_cons] at h₂
+          case cons head' tail' =>
+            simp only [List.map_cons, List.cons.injEq] at h₂
+            have ⟨h_head, h_tails ⟩ := h₂
+            rw [mapM_option_cons]
+            apply roundtrip₂
+            assumption
+            apply ih
+            simp only [List.cons.sizeOf_spec, Spec.Expr.call.sizeOf_spec] at h₁
+            somega
+            assumption
+    rw [List.mapM₁_eq_mapM]
+    rw [List.map₁_eq_map]
+    rw [inner]
+    simp only [Option.map_eq_map, Option.map_some', Option.some.injEq, Spec.Expr.set.injEq]
+    rfl
+    somega
+    rfl
+termination_by sizeOf e
+decreasing_by
+  all_goals simp_wf
+  all_goals (try omega)
+  all_goals (try (simp only [List.cons.sizeOf_spec, Spec.Expr.set.sizeOf_spec, Spec.Expr.call.sizeOf_spec] at h₁ <;> omega))
+  case _ =>
+    simp only [List.cons.sizeOf_spec, Spec.Expr.record.sizeOf_spec] at h₁
+    rename_i head' tail' _ h_eq' head as _
+    have size_step : sizeOf head'.snd  < sizeOf head' := by
+      cases head'
+      case _ =>
+        simp only [Prod.mk.sizeOf_spec]
+        omega
+    omega
